TotalExpressions.thy
@@ -1,11 +1,13 @@
 theory TotalExpressions
-imports Viper.ViperLang Viper.ValueAndBasicState TotalViperState Viper.Binop Viper.DeBruijn
+imports Viper.ViperLang Viper.ValueAndBasicState TotalViperState Viper.Binop Viper.DeBruijn Viper.PredicatesUtil TotalUtil
 begin
 
 (* duplicated: TODO share it *)
+(*
 fun the_address :: "'a val \<Rightarrow> address" where
   "the_address (VRef (Address a)) = a"
 | "the_address _ = undefined"
+*)
 
 fun the_rat :: "'a val \<Rightarrow> rat" where
   "the_rat (VPerm r) = r"
@@ -19,19 +21,167 @@ fun wd_binop :: "binop \<Rightarrow> 'a val \<Rightarrow> 'a val \<Rightarrow> b
   | "wd_binop Mod v1 v2 \<longleftrightarrow> v2 \<noteq> (VInt 0)"
   | "wd_binop _ _ _ = True"
 
-inductive red_pure_exp_total :: "program \<Rightarrow> 'a interp \<Rightarrow> pure_exp \<Rightarrow> 'a full_total_state \<Rightarrow> 'a extended_val \<Rightarrow> bool"
-  ("_, _ \<turnstile> ((\<langle>_;_\<rangle>) [\<Down>]\<^sub>t _)" [51,51,0,51,51] 81)
+datatype 'a standard_result = RMagic | RFailure | RNormal "'a full_total_state"
+
+definition get_valid_locs :: "'a full_total_state \<Rightarrow> heap_loc set"
+  where "get_valid_locs \<omega> = {l |l. pgt (get_mh_total_full \<omega> l) pnone}"
+
+
+definition inhale_perm_single :: "'a full_total_state \<Rightarrow> heap_loc \<Rightarrow> prat option \<Rightarrow> 'a full_total_state set"
+  where "inhale_perm_single \<omega> l p_opt =
+      {\<omega>'| \<omega>' q. 
+               option_fold ((=) q) (q \<noteq> pnone) p_opt \<and>
+               pgte pwrite (padd (get_mh_total_full \<omega> l) q) \<and>
+               \<omega>' = update_mask_total_full \<omega> ((get_mh_total_full \<omega>)(l := (padd (get_mh_total_full \<omega> l) q)))
+       }"
+
+definition inhale_perm_single_pred :: "'a full_total_state \<Rightarrow> 'a predicate_loc \<Rightarrow> prat option \<Rightarrow> 'a full_total_state set"
+  where "inhale_perm_single_pred \<omega> ploc p_opt = 
+      {\<omega>'| \<omega>' q.   
+               option_fold ((=) q) (q \<noteq> pnone) p_opt \<and>
+               pgte pwrite (padd (get_mp_total_full \<omega> ploc) q) \<and>
+               \<omega>' = update_pmask_total_full \<omega> ((get_mp_total_full \<omega>)(ploc := (padd (get_mp_total_full \<omega> ploc) q)))
+       }"
+
+fun inh_if_if_total :: "bool \<Rightarrow> bool \<Rightarrow> 'a full_total_state \<Rightarrow> 'a standard_result"  where
+  "inh_if_if_total False _ _ = RFailure"
+| "inh_if_if_total True False _ = RMagic"
+| "inh_if_if_total True True \<omega> = RNormal \<omega>"
+
+(* potential duplicate *)
+fun sub_expressions_exp_or_wildcard :: "pure_exp exp_or_wildcard \<Rightarrow> pure_exp set" where
+  "sub_expressions_exp_or_wildcard (PureExp e) = {e}"
+| "sub_expressions_exp_or_wildcard Wildcard = {}"
+
+(* TODO: duplicate with ViperLang.SemanticsPerm, put in some common theory *)
+fun sub_expressions_atomic :: "pure_exp atomic_assert \<Rightarrow> pure_exp set" where
+  "sub_expressions_atomic (Pure e) = {e}"
+| "sub_expressions_atomic (Acc x f p) = {x} \<union> sub_expressions_exp_or_wildcard p"
+| "sub_expressions_atomic (AccPredicate P exps p) = set exps \<union> sub_expressions_exp_or_wildcard p"
+
+text\<open>Pure expression evaluation, where the set of heap locations expresses the set of readable locations
+(if no set is provided, then all locations can be read).
+\<close>
+inductive red_pure_exp_total :: "program \<Rightarrow> 'a interp \<Rightarrow> (heap_loc set) option \<Rightarrow> pure_exp \<Rightarrow> 'a full_total_state \<Rightarrow> 'a extended_val \<Rightarrow> bool"
+  ("_, _, _ \<turnstile> ((\<langle>_;_\<rangle>) [\<Down>]\<^sub>t _)" [51,51,51,0,51,51] 81) and
+   red_pure_exps_total :: "program \<Rightarrow> 'a interp \<Rightarrow> (heap_loc set) option \<Rightarrow> pure_exp list \<Rightarrow> 'a full_total_state \<Rightarrow> ('a extended_val) list \<Rightarrow> bool" and
+   red_inhale :: "program \<Rightarrow>  'a interp \<Rightarrow> ('a full_total_state \<Rightarrow> bool) \<Rightarrow> assertion \<Rightarrow> 'a full_total_state \<Rightarrow> 'a standard_result \<Rightarrow> bool"
   for Pr :: program and \<Delta> :: "'a interp"
   where
-(* Independent of SA *)
-  RedLit: "Pr, \<Delta> \<turnstile> \<langle>ELit l; _\<rangle> [\<Down>]\<^sub>t Val (val_of_lit l)"
-| RedVar: "\<lbrakk> \<sigma> n = Some v \<rbrakk> \<Longrightarrow> Pr, \<Delta> \<turnstile> \<langle>Var n; (\<sigma>, _, _)\<rangle> [\<Down>]\<^sub>t Val v"
-| RedUnop: "\<lbrakk> Pr, \<Delta> \<turnstile> \<langle>e; \<omega>\<rangle> [\<Down>]\<^sub>t Val v ; eval_unop unop v = BinopNormal v' \<rbrakk> \<Longrightarrow> Pr, \<Delta> \<turnstile> \<langle>Unop unop e; \<omega>\<rangle> [\<Down>]\<^sub>t Val v'"
-| RedBinopLazy: "\<lbrakk> Pr, \<Delta> \<turnstile> \<langle>e1; \<omega>\<rangle> [\<Down>]\<^sub>t Val v1 ; eval_binop_lazy v1 bop = Some v \<rbrakk>
-  \<Longrightarrow> Pr, \<Delta> \<turnstile> \<langle>Binop e1 bop e2; \<omega>\<rangle> [\<Down>]\<^sub>t Val v"
-| RedBinop: "\<lbrakk> Pr, \<Delta> \<turnstile> \<langle>e1; \<omega>\<rangle> [\<Down>]\<^sub>t Val v1 ; Pr, \<Delta> \<turnstile> \<langle>e2; \<omega>\<rangle> [\<Down>]\<^sub>t Val v2 ; eval_binop_lazy v1 bop = None; eval_binop v1 bop v2 = BinopNormal v \<rbrakk>
-  \<Longrightarrow> Pr, \<Delta> \<turnstile> \<langle>Binop e1 bop e2; \<omega>\<rangle> [\<Down>]\<^sub>t Val v"
-(*| RedOld: "\<lbrakk> t l = Some \<phi> ; Pr, \<Delta> \<turnstile> \<langle>e; (\<sigma>, t, \<phi>)\<rangle> [\<Down>]\<^sub>t v \<rbrakk> \<Longrightarrow> Pr, \<Delta> \<turnstile> \<langle>Old l e; (\<sigma>, t, _)\<rangle> [\<Down>]\<^sub>t v"*) (* Implicitly propagates failures *)
+\<comment>\<open>Atomic inhale\<close>
+  InhAcc: 
+    "\<lbrakk> Pr, \<Delta>, Some (get_valid_locs \<omega>) \<turnstile> \<langle>e_r; \<omega>\<rangle> [\<Down>]\<^sub>t Val (VRef r); 
+       Pr, \<Delta>, Some (get_valid_locs \<omega>) \<turnstile> \<langle>e_p; \<omega>\<rangle> [\<Down>]\<^sub>t Val (VPerm p); 
+       W' = inhale_perm_single \<omega> (the_address r,f) (Some (Abs_prat p)) \<rbrakk> \<Longrightarrow>
+       red_inhale Pr \<Delta> R (Atomic (Acc e_r f (PureExp e_p))) \<omega> 
+                (inh_if_if_total (p \<ge> 0) (W' \<noteq> {} \<and> r \<noteq> Null) (SOME \<omega>'. \<omega>' \<in> W' \<and> R \<omega>'))"
+| InhAccPred:
+    "\<lbrakk> Pr, \<Delta>, Some (get_valid_locs \<omega>) \<turnstile> \<langle>e_p; \<omega>\<rangle> [\<Down>]\<^sub>t Val (VPerm p);
+       red_pure_exps_total Pr \<Delta> (Some (get_valid_locs \<omega>)) e_args \<omega> (map Val v_args);
+       W' = inhale_perm_single_pred \<omega> (pred_id, v_args) (Some (Abs_prat p)) \<rbrakk> \<Longrightarrow>       
+       red_inhale Pr \<Delta> R (Atomic (AccPredicate pred_id e_args (PureExp e_p))) \<omega> 
+                (inh_if_if_total (p \<ge> 0) (W' \<noteq> {} \<and> r \<noteq> Null) (SOME \<omega>'. \<omega>' \<in> W' \<and> R \<omega>'))"
+| InhAccWildcard: 
+    "\<lbrakk> Pr, \<Delta>, Some (get_valid_locs \<omega>) \<turnstile> \<langle>e_r; \<omega>\<rangle> [\<Down>]\<^sub>t Val (VRef r);
+       W' = inhale_perm_single \<omega> (the_address r,f) None \<rbrakk> \<Longrightarrow>
+       red_inhale Pr \<Delta> R (Atomic (Acc e_r f Wildcard)) \<omega> 
+                   (inh_if_if_total True (W' \<noteq> {} \<and> r \<noteq> Null) (SOME \<omega>'. \<omega>' \<in> W' \<and> R \<omega>'))"
+| InhAccPredWildcard: 
+    "\<lbrakk> Pr, \<Delta>, Some (get_valid_locs \<omega>) \<turnstile> \<langle>e_r; \<omega>\<rangle> [\<Down>]\<^sub>t Val (VRef r);
+       W' = inhale_perm_single_pred \<omega> (pred_id, v_args) None \<rbrakk> \<Longrightarrow>
+       red_inhale Pr \<Delta> R (Atomic (AccPredicate pred_id e_args Wildcard)) \<omega> 
+                 (inh_if_if_total True (W' \<noteq> {} \<and> r \<noteq> Null) (SOME \<omega>'. \<omega>' \<in> W' \<and> R \<omega>'))"
+| InhPureNormalMagic: 
+    "\<lbrakk> Pr, \<Delta>, Some (get_valid_locs \<omega>) \<turnstile> \<langle>e; \<omega>\<rangle> [\<Down>]\<^sub>t Val (VBool b) \<rbrakk> \<Longrightarrow>
+      red_inhale Pr \<Delta> R (Atomic (Pure e)) \<omega> (if b then RNormal \<omega> else RMagic)"
+| SubFailure: 
+    "\<lbrakk> e \<in> sub_expressions_atomic A; Pr, \<Delta>, Some (get_valid_locs \<omega>) \<turnstile> \<langle>e; \<omega>\<rangle> [\<Down>]\<^sub>t VFailure \<rbrakk> \<Longrightarrow> 
+      red_inhale Pr \<Delta>  R (Atomic A) \<omega> RFailure"
+
+\<comment>\<open>Connectives inhale\<close>
+| InhSepNormal: 
+   "\<lbrakk> red_inhale Pr \<Delta> R A \<omega> (RNormal \<omega>''); 
+      red_inhale Pr \<Delta> R B \<omega>'' res\<rbrakk> \<Longrightarrow>
+      red_inhale Pr \<Delta> R (A && B) \<omega> res"
+| InhSepFailureMagic:
+   "\<lbrakk> red_inhale Pr \<Delta> R A \<omega> resA; 
+      resA = RFailure \<or> resA = RMagic \<rbrakk> \<Longrightarrow>
+      red_inhale Pr \<Delta> R (A && B) \<omega> resA"
+| InhImpTrue:
+ "\<lbrakk> 
+    Pr, \<Delta>, Some (get_valid_locs \<omega>) \<turnstile> \<langle>e; \<omega>\<rangle> [\<Down>]\<^sub>t (Val (VBool True)); 
+    red_inhale Pr \<Delta> R A \<omega> res \<rbrakk> \<Longrightarrow>
+    red_inhale Pr \<Delta> R (Imp e A) \<omega> res"
+| InhImpFalse:
+ "\<lbrakk> Pr, \<Delta>, Some (get_valid_locs \<omega>) \<turnstile> \<langle>e; \<omega>\<rangle> [\<Down>]\<^sub>t Val (VBool False) \<rbrakk> \<Longrightarrow> 
+    red_inhale Pr \<Delta> R (Imp e A) \<omega> (RNormal \<omega>)"
+| InhImpFailure:
+ "\<lbrakk> Pr, \<Delta>, Some (get_valid_locs \<omega>) \<turnstile> \<langle>e; \<omega>\<rangle> [\<Down>]\<^sub>t VFailure \<rbrakk> \<Longrightarrow>
+   red_inhale Pr \<Delta> R (Imp e A) \<omega> RFailure"
+
+\<comment>\<open>Pure expression evaluation\<close>
+
+
+\<comment>\<open>Atomic expressions\<close>
+| RedLit: "Pr, \<Delta>, HLOpt \<turnstile> \<langle>ELit l; _\<rangle> [\<Down>]\<^sub>t Val (val_of_lit l)"
+| RedVar: "\<lbrakk> \<sigma> n = Some v \<rbrakk> \<Longrightarrow> Pr, \<Delta>, HLOpt \<turnstile> \<langle>Var n; (\<sigma>, _, _)\<rangle> [\<Down>]\<^sub>t Val v"
+| RedResult: "\<lbrakk> \<sigma> 0 = Some v \<rbrakk> \<Longrightarrow> Pr, \<Delta>, HLOpt \<turnstile> \<langle>Result; (\<sigma>, _, _)\<rangle> [\<Down>]\<^sub>t Val v"
+
+\<comment>\<open>Binop and Unop\<close>
+| RedBinopLazy: "\<lbrakk> Pr, \<Delta>, HLOpt \<turnstile> \<langle>e1; \<omega>\<rangle> [\<Down>]\<^sub>t Val v1 ; eval_binop_lazy v1 bop = Some v \<rbrakk>
+  \<Longrightarrow> Pr, \<Delta>, HLOpt \<turnstile> \<langle>Binop e1 bop e2; \<omega>\<rangle> [\<Down>]\<^sub>t Val v"
+| RedBinop: "\<lbrakk> Pr, \<Delta>, HLOpt \<turnstile> \<langle>e1; \<omega>\<rangle> [\<Down>]\<^sub>t Val v1 ; Pr, \<Delta>, HLOpt \<turnstile> \<langle>e2; \<omega>\<rangle> [\<Down>]\<^sub>t Val v2 ; eval_binop_lazy v1 bop = None; eval_binop v1 bop v2 = BinopNormal v \<rbrakk>
+  \<Longrightarrow> Pr, \<Delta>, HLOpt \<turnstile> \<langle>Binop e1 bop e2; \<omega>\<rangle> [\<Down>]\<^sub>t Val v"
+| RedBinopRightFailure: "\<lbrakk> Pr, \<Delta>, HLOpt \<turnstile> \<langle>e1; \<omega>\<rangle> [\<Down>]\<^sub>t Val v1; Pr, \<Delta>, HLOpt \<turnstile> \<langle>e2; \<omega>\<rangle> [\<Down>]\<^sub>t VFailure;  eval_binop_lazy v1 bop = None \<rbrakk>
+  \<Longrightarrow> Pr, \<Delta>, HLOpt \<turnstile> \<langle>Binop e1 bop e2; \<omega>\<rangle> [\<Down>]\<^sub>t VFailure"
+| RedBinopOpFailure: "\<lbrakk> Pr, \<Delta>, HLOpt \<turnstile> \<langle>e1; \<omega>\<rangle> [\<Down>]\<^sub>t Val v1 ; Pr, \<Delta>, HLOpt \<turnstile> \<langle>e2; \<omega>\<rangle> [\<Down>]\<^sub>t Val v2 ; eval_binop v1 bop v2 = BinopOpFailure ; eval_binop_lazy v1 bop = None \<rbrakk>
+  \<Longrightarrow> Pr, \<Delta>, HLOpt \<turnstile> \<langle>Binop e1 bop e2; \<omega>\<rangle> [\<Down>]\<^sub>t VFailure" (* Division by 0 *)
+| RedBinopLeftFailure: "\<lbrakk> Pr, \<Delta>, HLOpt \<turnstile> \<langle>e1; \<omega>\<rangle> [\<Down>]\<^sub>t VFailure \<rbrakk>
+  \<Longrightarrow> Pr, \<Delta>, HLOpt \<turnstile> \<langle>Binop e1 bop e2; \<omega>\<rangle> [\<Down>]\<^sub>t VFailure" (* could be replaced *)
+
+| RedUnop: "\<lbrakk> Pr, \<Delta>, HLOpt \<turnstile> \<langle>e; \<omega>\<rangle> [\<Down>]\<^sub>t Val v; eval_unop unop v = BinopNormal v' \<rbrakk> \<Longrightarrow> Pr, \<Delta>, HLOpt \<turnstile> \<langle>Unop unop e; \<omega>\<rangle> [\<Down>]\<^sub>t Val v'"
+| RedUnopFailure: "\<lbrakk> Pr, \<Delta>, HLOpt \<turnstile> \<langle>e; \<omega>\<rangle> [\<Down>]\<^sub>t VFailure \<rbrakk> \<Longrightarrow> Pr, \<Delta>, HLOpt \<turnstile> \<langle>Unop unop e; \<omega>\<rangle> [\<Down>]\<^sub>t VFailure" (* could be replaced *)
+
+\<comment>\<open>Cond\<close>
+| RedCondExpTrue: "\<lbrakk> Pr, \<Delta>, HLOpt \<turnstile> \<langle>e1; \<omega>\<rangle> [\<Down>]\<^sub>t Val (VBool True) ; Pr, \<Delta>, HLOpt \<turnstile> \<langle>e2; \<omega>\<rangle> [\<Down>]\<^sub>t r \<rbrakk>
+  \<Longrightarrow> Pr, \<Delta>, HLOpt \<turnstile> \<langle>CondExp e1 e2 e3; \<omega>\<rangle> [\<Down>]\<^sub>t r"
+| RedCondExpFalse: "\<lbrakk> Pr, \<Delta>, HLOpt \<turnstile> \<langle>e1; \<omega>\<rangle> [\<Down>]\<^sub>t Val (VBool False) ; Pr, \<Delta>, HLOpt \<turnstile> \<langle>e3; \<omega>\<rangle> [\<Down>]\<^sub>t r \<rbrakk>
+  \<Longrightarrow> Pr, \<Delta>, HLOpt \<turnstile> \<langle>CondExp e1 e2 e3; \<omega>\<rangle> [\<Down>]\<^sub>t r"
+| RedCondExpFailure: "\<lbrakk> Pr, \<Delta>, HLOpt \<turnstile> \<langle>e1; \<omega>\<rangle> [\<Down>]\<^sub>t VFailure \<rbrakk>
+  \<Longrightarrow> Pr, \<Delta>, HLOpt \<turnstile> \<langle>CondExp e1 e2 e3; \<omega>\<rangle> [\<Down>]\<^sub>t VFailure" (* could be replaced *)
+
+\<comment>\<open>Old\<close>
+| RedOld: "\<lbrakk> t l = Some \<phi> ; Pr, \<Delta>, HLOpt \<turnstile> \<langle>e; (\<sigma>, t, \<phi>)\<rangle> [\<Down>]\<^sub>t v \<rbrakk> \<Longrightarrow> Pr, \<Delta>, HLOpt \<turnstile> \<langle>Old l e; (\<sigma>, t, _)\<rangle> [\<Down>]\<^sub>t v"
+| RedOldFailure: "\<lbrakk> t l = None \<rbrakk> \<Longrightarrow> Pr, \<Delta>, HLOpt \<turnstile> \<langle>Old l e ; (_, t, _)\<rangle> [\<Down>]\<^sub>t VFailure" 
+
+\<comment>\<open>Heap lookup\<close>
+| RedField: "\<lbrakk> Pr, \<Delta>, HLOpt \<turnstile> \<langle>e; \<omega>\<rangle> [\<Down>]\<^sub>t Val (VRef (Address a)) ; get_heap_total_full \<omega> (a, f) = v \<rbrakk> \<Longrightarrow> 
+       Pr, \<Delta>, HLOpt \<turnstile> \<langle>FieldAcc e f; \<omega>\<rangle> [\<Down>]\<^sub>t option_fold (\<lambda>l. if (a,f) \<in> l then Val v else VFailure) (Val v) HLOpt"
+| RedFieldFailure: "\<lbrakk> Pr, \<Delta>, HLOpt \<turnstile> \<langle>e; \<omega>\<rangle> [\<Down>]\<^sub>t VFailure \<rbrakk> \<Longrightarrow> Pr, \<Delta>, HLOpt \<turnstile> \<langle>FieldAcc e f; \<omega>\<rangle> [\<Down>]\<^sub>t VFailure" (* could be replaced *)
+
+\<comment>\<open>Permission introspection\<close>
+| RedPermNull: "\<lbrakk> Pr, \<Delta>, HLOpt \<turnstile> \<langle>e; \<omega>\<rangle> [\<Down>]\<^sub>t Val (VRef Null) \<rbrakk> \<Longrightarrow> Pr, \<Delta>, HLOpt \<turnstile> \<langle>Perm e f; \<omega>\<rangle> [\<Down>]\<^sub>t Val (VPerm 0)"
+| RedPerm: "\<lbrakk> Pr, \<Delta>, HLOpt \<turnstile> \<langle>e; \<omega>\<rangle> [\<Down>]\<^sub>t Val (VRef (Address a)) \<rbrakk> \<Longrightarrow> Pr, \<Delta>, HLOpt \<turnstile> \<langle>Perm e f; \<omega>\<rangle> [\<Down>]\<^sub>t Val (VPerm (Rep_prat (get_mask_total_full \<omega> (a, f))))"
+| RedPermFailure: "\<lbrakk> Pr, \<Delta>, HLOpt \<turnstile> \<langle>e; \<omega>\<rangle> [\<Down>]\<^sub>t VFailure \<rbrakk> \<Longrightarrow> Pr, \<Delta>, HLOpt \<turnstile> \<langle>Perm e f; \<omega>\<rangle> [\<Down>]\<^sub>t VFailure" (* could be replaced *)
+(*
+\<comment>\<open>Unfolding\<close>
+| RedUnfolding: "\<lbrakk> 
+         Pr, \<Delta>, HLOpt \<turnstile> \<langle>e_arg; \<omega>\<rangle> [\<Down>]\<^sub>t v_arg;
+        ViperLang.predicates Pr p = Some pred;
+        ViperLang.predicate_decl.body pred = Some pred_body;
+        red_inhale Pr \<Delta> False pred_body \<omega> (RNormal \<omega>');
+            
+ \<rbrakk> \<Longrightarrow>
+     Pr, \<Delta>, HLOpt \<turnstile> \<langle>Unfolding p [e_arg] p_body; \<omega>\<rangle> [\<Down>]\<^sub>t Val (VPerm 0)"
+*)
+
+(*| RedPropagateFailure: "\<lbrakk> e \<in> sub_pure_exp e' ; Pr, \<Delta> \<turnstile> \<langle>e; \<omega>\<rangle> [\<Down>]\<^sub>t VFailure \<rbrakk> \<Longrightarrow>  Pr, \<Delta> \<turnstile> \<langle>e'; \<omega>\<rangle> [\<Down>]\<^sub>t VFailure"*)
+(*| RedUnfoldingPermNegFailure: "\<lbrakk> Pr, \<Delta> \<turnstile> \<langle>f; \<omega>\<rangle> [\<Down>]\<^sub>t Val (VPerm v) ; v < 0 \<rbrakk> \<Longrightarrow> Pr, \<Delta> \<turnstile> \<langle>Unfolding p exps f e; \<omega>\<rangle> [\<Down>]\<^sub>t VFailure"*)
+(*
+(* perm(P(...)) = 0 if equirecursive *)
+| RedPermPred: "\<lbrakk> list_all2 (\<lambda>e v. Pr, \<Delta> \<turnstile> \<langle>e; \<omega>\<rangle> [\<Down>] Val v) exps vals \<rbrakk>
+  \<Longrightarrow> Pr, \<Delta> \<turnstile> \<langle>PermPred p exps; \<omega>\<rangle> [\<Down>] Val (VPerm (Rep_prat (get_pm \<omega> (p, vals))))"
+*)
 (*| RedLet: "\<lbrakk> Pr, \<Delta> \<turnstile> \<langle>e1; \<omega>\<rangle> [\<Down>]\<^sub>t Val v1 ; Pr, \<Delta> \<turnstile> \<langle>e2; shift_and_add_state \<omega> v1\<rangle> [\<Down>]\<^sub>t r \<rbrakk> \<Longrightarrow> Pr, \<Delta> \<turnstile> \<langle>Let e1 e2; \<omega>\<rangle> [\<Down>]\<^sub>t r"
 | RedExistsTrue: "\<lbrakk> v \<in> set_from_type \<Delta> ty ; Pr, \<Delta> \<turnstile> \<langle>e; shift_and_add_state \<omega> v\<rangle> [\<Down>]\<^sub>t Val (VBool True) ;
   \<And>v'. \<exists>b. Pr, \<Delta> \<turnstile> \<langle>e; shift_and_add_state \<omega> v'\<rangle> [\<Down>]\<^sub>t Val (VBool b) \<rbrakk>
@@ -42,37 +192,118 @@ inductive red_pure_exp_total :: "program \<Rightarrow> 'a interp \<Rightarrow> p
   \<Longrightarrow> Pr, \<Delta> \<turnstile> \<langle>PForall ty e; \<omega>\<rangle> [\<Down>]\<^sub>t Val (VBool True)"
 | RedForallFalse: "\<lbrakk> v \<in> set_from_type \<Delta> ty ; Pr, \<Delta> \<turnstile> \<langle>e; shift_and_add_state \<omega> v\<rangle> [\<Down>]\<^sub>t Val (VBool False) \<rbrakk>
   \<Longrightarrow> Pr, \<Delta> \<turnstile> \<langle>PForall ty e; \<omega>\<rangle> [\<Down>]\<^sub>t Val (VBool False)"*)
-| RedCondExpTrue: "\<lbrakk> Pr, \<Delta> \<turnstile> \<langle>e1; \<omega>\<rangle> [\<Down>]\<^sub>t Val (VBool True) ; Pr, \<Delta> \<turnstile> \<langle>e2; \<omega>\<rangle> [\<Down>]\<^sub>t r \<rbrakk>
-  \<Longrightarrow> Pr, \<Delta> \<turnstile> \<langle>CondExp e1 e2 e3; \<omega>\<rangle> [\<Down>]\<^sub>t r"
-| RedCondExpFalse: "\<lbrakk> Pr, \<Delta> \<turnstile> \<langle>e1; \<omega>\<rangle> [\<Down>]\<^sub>t Val (VBool False) ; Pr, \<Delta> \<turnstile> \<langle>e3; \<omega>\<rangle> [\<Down>]\<^sub>t r \<rbrakk>
-  \<Longrightarrow> Pr, \<Delta> \<turnstile> \<langle>CondExp e1 e2 e3; \<omega>\<rangle> [\<Down>]\<^sub>t r"
-| RedPermNull: "\<lbrakk> Pr, \<Delta> \<turnstile> \<langle>e; \<omega>\<rangle> [\<Down>]\<^sub>t Val (VRef Null) \<rbrakk> \<Longrightarrow> Pr, \<Delta> \<turnstile> \<langle>Perm e f; \<omega>\<rangle> [\<Down>]\<^sub>t Val (VPerm 0)"
-| RedResult: "\<lbrakk> \<sigma> 0 = Some v \<rbrakk> \<Longrightarrow> Pr, \<Delta> \<turnstile> \<langle>Result; (\<sigma>, _, _)\<rangle> [\<Down>]\<^sub>t Val v"
-(*| RedUnfoldingPermNegFailure: "\<lbrakk> Pr, \<Delta> \<turnstile> \<langle>f; \<omega>\<rangle> [\<Down>]\<^sub>t Val (VPerm v) ; v < 0 \<rbrakk> \<Longrightarrow> Pr, \<Delta> \<turnstile> \<langle>Unfolding p exps f e; \<omega>\<rangle> [\<Down>]\<^sub>t VFailure"*)
-
-| RedBinopRightFailure: "\<lbrakk> Pr, \<Delta> \<turnstile> \<langle>e1; \<omega>\<rangle> [\<Down>]\<^sub>t Val v1 ; Pr, \<Delta> \<turnstile> \<langle>e2; \<omega>\<rangle> [\<Down>]\<^sub>t VFailure ;  eval_binop_lazy v1 bop = None \<rbrakk>
-  \<Longrightarrow> Pr, \<Delta> \<turnstile> \<langle>Binop e1 bop e2; \<omega>\<rangle> [\<Down>]\<^sub>t VFailure"
-| RedBinopFailure: "\<lbrakk> Pr, \<Delta> \<turnstile> \<langle>e1; \<omega>\<rangle> [\<Down>]\<^sub>t Val v1 ; Pr, \<Delta> \<turnstile> \<langle>e2; \<omega>\<rangle> [\<Down>]\<^sub>t Val v2 ; eval_binop v1 bop v2 = BinopOpFailure ; eval_binop_lazy v1 bop = None \<rbrakk>
-  \<Longrightarrow> Pr, \<Delta> \<turnstile> \<langle>Binop e1 bop e2; \<omega>\<rangle> [\<Down>]\<^sub>t VFailure" (* Division by 0 *)
-| RedOldFailure: "\<lbrakk> t l = None \<rbrakk> \<Longrightarrow> Pr, \<Delta> \<turnstile> \<langle>Old l e ; (_, t, _)\<rangle> [\<Down>]\<^sub>t VFailure"
 (*
 | RedExistsFailure: "\<lbrakk> v \<in> set_from_type \<Delta> ty \<longrightarrow> Pr, \<Delta> \<turnstile> \<langle>e; shift_and_add_state \<omega> v\<rangle> [\<Down>]\<^sub>t VFailure \<rbrakk>
   \<Longrightarrow> Pr, \<Delta> \<turnstile> \<langle>PExists ty e; \<omega>\<rangle> [\<Down>]\<^sub>t VFailure"
 | RedForallFailure: "\<lbrakk> v \<in> set_from_type \<Delta> ty \<longrightarrow> Pr, \<Delta> \<turnstile> \<langle>e; shift_and_add_state \<omega> v\<rangle> [\<Down>]\<^sub>t VFailure \<rbrakk>
   \<Longrightarrow> Pr, \<Delta> \<turnstile> \<langle>PForall ty e; \<omega>\<rangle> [\<Down>]\<^sub>t VFailure"*)
-| RedPropagateFailure: "\<lbrakk> e \<in> sub_pure_exp e' ; Pr, \<Delta> \<turnstile> \<langle>e; \<omega>\<rangle> [\<Down>]\<^sub>t VFailure \<rbrakk> \<Longrightarrow>  Pr, \<Delta> \<turnstile> \<langle>e'; \<omega>\<rangle> [\<Down>]\<^sub>t VFailure"
 
-(* Dependent on the SA *)
-| RedField: "\<lbrakk> Pr, \<Delta> \<turnstile> \<langle>e; \<omega>\<rangle> [\<Down>]\<^sub>t Val (VRef (Address a)) ; get_heap_total_full \<omega> (a, f) = v \<rbrakk> \<Longrightarrow> Pr, \<Delta> \<turnstile> \<langle>FieldAcc e f; \<omega>\<rangle> [\<Down>]\<^sub>t Val v"
-| RedPerm: "\<lbrakk> Pr, \<Delta> \<turnstile> \<langle>e; \<omega>\<rangle> [\<Down>]\<^sub>t Val (VRef (Address a)) \<rbrakk> \<Longrightarrow> Pr, \<Delta> \<turnstile> \<langle>Perm e f; \<omega>\<rangle> [\<Down>]\<^sub>t Val (VPerm (Rep_prat (get_mask_total_full \<omega> (a, f))))"
-(*
-(* perm(P(...)) = 0 if equirecursive *)
-| RedPermPred: "\<lbrakk> list_all2 (\<lambda>e v. Pr, \<Delta> \<turnstile> \<langle>e; \<omega>\<rangle> [\<Down>] Val v) exps vals \<rbrakk>
-  \<Longrightarrow> Pr, \<Delta> \<turnstile> \<langle>PermPred p exps; \<omega>\<rangle> [\<Down>] Val (VPerm (Rep_prat (get_pm \<omega> (p, vals))))"
+
+
+inductive unfold_rel :: "program \<Rightarrow> 'a interp \<Rightarrow> predicate_ident \<Rightarrow> ('a val list) \<Rightarrow> prat \<Rightarrow> 'a full_total_state \<Rightarrow> 'a full_total_state \<Rightarrow> bool"
+  where UnfoldRelStep: 
+                    "\<lbrakk> ViperLang.predicates Pr pred_id = Some pred_decl;
+                     ViperLang.predicate_decl.body pred_decl = Some pred_body;
+                     m = get_pmask_total_full \<omega>;
+                     pgte (m (pred_id,vs)) q;
+                     m' = m( (pred_id,vs) := psub (m (pred_id, vs)) q);
+                     \<omega>2 = (nth_option vs, get_trace_total \<omega>, update_pmask_total (get_mh_total_full \<omega>) m');
+                     red_inhale Pr \<Delta> (\<lambda>_. True) (syntactic_mult (Rep_prat q) pred_body) \<omega>2 (RNormal \<omega>') \<rbrakk> \<Longrightarrow> 
+                     unfold_rel Pr \<Delta> pred_id vs q \<omega> \<omega>'"
+
+definition unfold_rel_general
+  where "unfold_rel_general Pr \<Delta> \<omega> \<omega>' \<equiv> \<exists> pred_id vs q. unfold_rel Pr \<Delta> pred_id vs q \<omega> \<omega>'"
+
+definition unfold_rel_multi
+  where "unfold_rel_multi Pr \<Delta>  \<equiv> rtranclp (unfold_rel_general Pr \<Delta>)"
+
+coinductive unfold_consistent :: "program \<Rightarrow> 'a interp \<Rightarrow> 'a full_total_state \<Rightarrow> bool"
+  where 
+  unfold_step: "\<lbrakk> \<And> pred_id vs q. pgt (get_pmask_total_full \<omega> (pred_id,vs)) q \<Longrightarrow>
+                     \<exists>\<omega>'. unfold_rel Pr \<Delta> pred_id vs q \<omega> \<omega>' \<and> unfold_consistent Pr \<Delta> \<omega>' \<rbrakk> \<Longrightarrow>
+                  unfold_consistent Pr \<Delta> \<omega>"
+
+(*  this definition here is incorrect since it does not account for non-determinism
+definition unfold_consistent where
+ "unfold_consistent Pr \<Delta> \<omega> \<equiv> 
+          \<forall> \<omega>' pred_id vs q. 
+               (unfold_rel_multi Pr \<Delta> \<omega> \<omega>' \<and> pgt (get_pmask_total_full \<omega>' (pred_id,vs)) q) \<longrightarrow>
+               (\<exists>\<omega>''. unfold_rel Pr \<Delta> pred_id vs q \<omega>' \<omega>'')"
 *)
 
-datatype inh_exh_conf = CInhale | CExhale "heap_loc set"
+text \<open>Expression evaluation as a function. Using this function makes sense, when it is known that 
+e is well-defined and is deterministic (for example, if e is the body of a predicate)\<close>
+fun red_pure_exp_total_fun :: "program \<Rightarrow> 'a interp \<Rightarrow> pure_exp \<Rightarrow> 'a full_total_state \<Rightarrow> 'a val"
+  where "red_pure_exp_total_fun Pr \<Delta> e \<omega> = (SOME v. Pr, \<Delta>, None \<turnstile> \<langle>e; \<omega>\<rangle> [\<Down>]\<^sub>t Val v)"
 
+fun red_pure_exps_total_fun :: "program \<Rightarrow> 'a interp \<Rightarrow> pure_exp list \<Rightarrow> 'a full_total_state \<Rightarrow> ('a val) list"
+  where "red_pure_exps_total_fun Pr \<Delta> es \<omega> = (SOME vs. red_pure_exps_total Pr \<Delta> None es \<omega> (map Val vs))"
+
+fun extract_address_from_val :: "'a val \<Rightarrow> address"
+  where 
+    "extract_address_from_val (VRef (Address a)) = a"
+  | "extract_address_from_val _ = undefined"
+
+fun extract_perm_from_val :: "'a val \<Rightarrow> rat"
+  where 
+    "extract_perm_from_val (VPerm r) = r"
+  | "extract_perm_from_val _ = undefined"
+
+fun is_positive_permission :: "program \<Rightarrow> 'a interp \<Rightarrow> pure_exp exp_or_wildcard \<Rightarrow> 'a full_total_state \<Rightarrow> bool"
+  where 
+    "is_positive_permission Pr \<Delta> Wildcard \<omega> = True"
+  | "is_positive_permission Pr \<Delta> (PureExp e) \<omega> = (extract_perm_from_val (red_pure_exp_total_fun Pr \<Delta> e \<omega>) > 0)"
+
+
+fun assertion_heap_snapshot :: "program \<Rightarrow> 'a interp \<Rightarrow> assertion \<Rightarrow> 'a full_total_state \<Rightarrow> heap_loc set"
+  where 
+   "assertion_heap_snapshot Pr \<Delta> (Atomic (Pure e)) \<omega> = {}"
+ | "assertion_heap_snapshot Pr \<Delta> (Atomic (Acc e f e_p)) \<omega> = 
+             (if is_positive_permission Pr \<Delta> e_p \<omega> then 
+                  {(extract_address_from_val (red_pure_exp_total_fun Pr \<Delta> e \<omega>), f)} 
+              else {})"
+ | "assertion_heap_snapshot Pr \<Delta> (Atomic (AccPredicate pred_id e_args e_p)) \<omega> = 
+             (if is_positive_permission Pr \<Delta> e_p \<omega> then
+                fst (get_pheap_total_full \<omega> (pred_id, red_pure_exps_total_fun Pr \<Delta> e_args \<omega>))
+              else {})"
+ | "assertion_heap_snapshot Pr \<Delta> (Imp e A) \<omega> =
+             (if red_pure_exp_total_fun Pr \<Delta> e \<omega> = VBool True then 
+                 assertion_heap_snapshot Pr \<Delta> A \<omega> 
+              else {})"
+ | "assertion_heap_snapshot Pr \<Delta> (A && B) \<omega> = assertion_heap_snapshot Pr \<Delta> A \<omega> \<union> assertion_heap_snapshot Pr \<Delta> B \<omega>"      
+ | "assertion_heap_snapshot Pr \<Delta> _ \<omega> = undefined" (* wands and quantified permissions not supported *)
+
+fun assertion_predicate_snapshot :: "program \<Rightarrow> 'a interp \<Rightarrow> assertion \<Rightarrow> 'a full_total_state \<Rightarrow> 'a predicate_loc set"
+  where 
+   "assertion_predicate_snapshot Pr \<Delta> (Atomic (Pure e)) \<omega> = {}"
+ | "assertion_predicate_snapshot Pr \<Delta> (Atomic (Acc e f e_p)) \<omega> = {}"
+ | "assertion_predicate_snapshot Pr \<Delta> (Atomic (AccPredicate pred_id e_args e_p)) \<omega> = 
+             (if is_positive_permission Pr \<Delta> e_p \<omega> then
+                {(pred_id, red_pure_exps_total_fun Pr \<Delta> e_args \<omega>)} \<union> 
+                snd (get_pheap_total_full \<omega> (pred_id, red_pure_exps_total_fun Pr \<Delta> e_args \<omega>))
+              else {})"
+ | "assertion_predicate_snapshot Pr \<Delta> (Imp e A) \<omega> =
+             (if red_pure_exp_total_fun Pr \<Delta> e \<omega> = VBool True then 
+                 assertion_predicate_snapshot Pr \<Delta> A \<omega> 
+              else {})"
+ | "assertion_predicate_snapshot Pr \<Delta> (A && B) \<omega> = assertion_predicate_snapshot Pr \<Delta> A \<omega> \<union> assertion_predicate_snapshot Pr \<Delta> B \<omega>"      
+ | "assertion_predicate_snapshot Pr \<Delta> _ \<omega> = undefined" (* wands and quantified permissions not supported *)
+
+
+definition pheap_consistent :: "program \<Rightarrow> 'a interp \<Rightarrow> 'a full_total_state \<Rightarrow> bool" where
+ "pheap_consistent Pr \<Delta> \<omega> \<equiv> 
+          \<forall> \<omega>' pred_id vs pred_decl. 
+               (unfold_rel_multi Pr \<Delta> \<omega> \<omega>' \<and> pgt (get_pmask_total_full \<omega>' (pred_id,vs)) pnone \<and>
+                ViperLang.predicates Pr pred_id = Some pred_decl) \<longrightarrow>
+                option_fold (\<lambda> pred_body. get_pheap_total_full \<omega> (pred_id, vs) = 
+                              (assertion_heap_snapshot Pr \<Delta> pred_body \<omega>, assertion_predicate_snapshot Pr \<Delta> pred_body \<omega>) )
+                            True
+                            (ViperLang.predicate_decl.body pred_decl)"
+
+
+
+datatype inh_exh_conf = CInhale | CExhale "heap_loc set"
+(*
 (* can't show this, since need to take typing into account *)
 lemma wd_binop_total: 
   assumes "wd_binop bop v1 v2"
@@ -107,6 +338,7 @@ fun wd_pure_exp_total :: "program \<Rightarrow> 'a interp \<Rightarrow> inh_exh_
 | "wd_pure_exp_total conf Pr \<Delta> (Let e1 e2) \<omega> \<longleftrightarrow> False"
 | "wd_pure_exp_total conf Pr \<Delta> (PExists ty e) \<omega> \<longleftrightarrow> False"
 | "wd_pure_exp_total conf Pr \<Delta> (PForall ty e) \<omega> \<longleftrightarrow> False" 
+*)
 *)
 
 end
