TotalSemantics.thy
@@ -3,192 +3,104 @@ imports Viper.ViperLang TotalExpressions "HOL-Eisbach.Eisbach" "HOL-Eisbach.Eisb
 begin
 
 (*datatype 'a result = Failure | Set (select_set: "'a full_total_state set")*)
-datatype 'a standard_result = RMagic | RFailure | RNormal "'a full_total_state"
 
 
-definition inhale_perm_single :: "bool \<Rightarrow>'a full_total_state \<Rightarrow> heap_loc \<Rightarrow> prat option \<Rightarrow> 'a full_total_state set"
-  where "inhale_perm_single havoc_new \<omega> l p_opt =
-      {\<omega>'| \<omega>' q v. get_store_total \<omega>' = get_store_total \<omega> \<and>
-               get_trace_total \<omega>' = get_trace_total \<omega> \<and>
-               option_fold ((=) q) (q \<noteq> pnone) p_opt \<and>
-               pgte pwrite (padd (get_mask_total_full \<omega> l) q) \<and>
-               get_mask_total_full \<omega>' = (get_mask_total_full \<omega>)(l := (padd (get_mask_total_full \<omega> l) q)) \<and>               
-               get_heap_total_full \<omega>' =
-                   (if havoc_new \<and> (get_mask_total_full \<omega> l) = pnone then 
-                      (get_heap_total_full \<omega>)(l := v) 
-                    else
-                       get_heap_total_full \<omega>)
-       }"
-
-
-inductive red_inhale :: "program \<Rightarrow> 'a interp \<Rightarrow> bool \<Rightarrow> assertion \<Rightarrow> 'a full_total_state \<Rightarrow>  'a standard_result \<Rightarrow> bool"
-  for Pr :: program and \<Delta> :: "'a interp" and havoc_new :: bool
-  where 
-  (** sep. conj **)
-   InhSepNormal: 
-   "\<lbrakk> red_inhale Pr \<Delta> havoc_new A \<omega> (RNormal \<omega>''); 
-      red_inhale Pr \<Delta> havoc_new B \<omega>'' res\<rbrakk> \<Longrightarrow>
-      red_inhale Pr \<Delta> havoc_new (A && B) \<omega> res"
- | InhSepFailureMagic: 
-   "\<lbrakk> red_inhale Pr \<Delta> havoc_new A \<omega> resA; 
-      resA = RFailure \<or> resA = RMagic \<rbrakk> \<Longrightarrow>
-      red_inhale Pr \<Delta> havoc_new (A && B) \<omega> resA"
-  (** if-else **)
- | InhImpTrue: 
-   "\<lbrakk> wd_pure_exp_total Pr \<Delta> CInhale e \<omega>; 
-      Pr, \<Delta> \<turnstile> \<langle>e; \<omega>\<rangle> [\<Down>]\<^sub>t (Val (VBool True)); 
-      red_inhale Pr \<Delta> havoc_new A \<omega> res \<rbrakk> \<Longrightarrow>
-      red_inhale Pr \<Delta> havoc_new (Imp e A) \<omega> res" 
- | InhImpFalse:  
-   "\<lbrakk> wd_pure_exp_total Pr \<Delta> CInhale e \<omega>; 
-      Pr, \<Delta> \<turnstile> \<langle>e; \<omega>\<rangle> [\<Down>]\<^sub>t Val (VBool False) \<rbrakk> \<Longrightarrow> 
-      red_inhale Pr \<Delta> havoc_new (Imp e A) \<omega> (RNormal \<omega>)"
- | InhImpFailure: 
-   "\<lbrakk> \<not> wd_pure_exp_total Pr \<Delta> CInhale e \<omega> \<rbrakk> \<Longrightarrow> 
-     red_inhale Pr \<Delta> havoc_new (Imp e A) \<omega>  RFailure"
-(** inhale/assume acc(e.f, p) **) (* Pr, \<Delta> \<turnstile> \<langle>ELit l; _\<rangle> [\<Down>]\<^sub>t Val (val_of_lit l) *)
-(* \<omega>' \<in> plus_total_full_set {\<omega>} 
-                        ((singleton_total havoc_new (a,f) (Abs_prat p) (get_heap_total_full \<omega> (a,f)) (get_store_total \<omega>) (get_trace_total \<omega>)))*)
- | InhAcc: 
-    "\<lbrakk> Pr, \<Delta> \<turnstile> \<langle>e_r; \<omega>\<rangle> [\<Down>]\<^sub>t Val (VRef (Address a)); Pr, \<Delta> \<turnstile> \<langle>e_p; \<omega>\<rangle> [\<Down>]\<^sub>t Val (VPerm p); p \<ge> 0; 
-       wd_pure_exp_total Pr \<Delta> CInhale e_r \<omega>;
-       wd_pure_exp_total Pr \<Delta> CInhale e_p \<omega>;
-       \<omega>' \<in> inhale_perm_single havoc_new \<omega> (a,f) (Some (Abs_prat p))\<rbrakk> \<Longrightarrow>
-       red_inhale Pr \<Delta> havoc_new (Atomic (Acc e_r f (PureExp e_p))) \<omega> (RNormal \<omega>')"
- | InhAssumeAccFail1: 
-    "\<lbrakk> Pr, \<Delta> \<turnstile> \<langle>e_r; \<omega>\<rangle> [\<Down>]\<^sub>t Val (VRef Null) \<rbrakk> \<Longrightarrow> 
-      red_inhale Pr \<Delta> havoc_new (Atomic (Acc e_r f (PureExp e_p))) \<omega> RMagic"
- | InhAssumeAccFail2: 
-    "\<lbrakk> Pr, \<Delta> \<turnstile> \<langle>e_r; \<omega>\<rangle> [\<Down>]\<^sub>t Val (VRef (Address a)); Pr, \<Delta> \<turnstile> \<langle>e_p; \<omega>\<rangle> [\<Down>]\<^sub>t Val (VPerm p); 
-      (\<not>wd_pure_exp_total Pr \<Delta> CInhale e_r \<omega> \<or> \<not>wd_pure_exp_total Pr \<Delta> CInhale e_r \<omega> \<or> p < 0)\<rbrakk> \<Longrightarrow>
-      red_inhale Pr \<Delta> havoc_new (Atomic (Acc e_r f (PureExp e_p))) \<omega> RFailure"
-(** inhale/assume acc(e.f, wildcard) **)
-(*  \<omega>' \<in> plus_total_full_set {\<omega>} 
-        singleton_total_wildcard havoc_new (r,f) (get_heap_total_full \<omega> (r,f)) (get_store_total \<omega>) (get_trace_total \<omega>)) *)
- | InhAccWildcard: 
-    "\<lbrakk> Pr, \<Delta> \<turnstile> \<langle>e_r; \<omega>\<rangle> [\<Down>]\<^sub>t Val (VRef (Address a));
-       (wd_pure_exp_total Pr \<Delta> CInhale e_r \<omega>);
-       \<omega>' \<in> inhale_perm_single havoc_new \<omega> (a,f) None \<rbrakk> \<Longrightarrow>
-       red_inhale Pr \<Delta> havoc_new (Atomic (Acc e_r f Wildcard)) \<omega> (RNormal \<omega>')"
-  | InhAssumeAccWildcardFail1: 
-    "\<lbrakk> Pr, \<Delta> \<turnstile> \<langle>e_r; \<omega>\<rangle> [\<Down>]\<^sub>t Val (VRef Null) \<rbrakk> \<Longrightarrow> 
-    red_inhale Pr \<Delta> havoc_new (Atomic (Acc e_r f Wildcard)) \<omega> RMagic"
- | InhAssumeAccWildcardFail2: 
-     "\<lbrakk> Pr, \<Delta> \<turnstile> \<langle>e_r; \<omega>\<rangle> [\<Down>]\<^sub>t Val (VRef (Address a)); 
-        Pr, \<Delta> \<turnstile> \<langle>e_p; \<omega>\<rangle> [\<Down>]\<^sub>t Val (VPerm p); 
-       \<not>wd_pure_exp_total Pr \<Delta> CInhale e_r \<omega>\<rbrakk> \<Longrightarrow>
-    red_inhale Pr \<Delta> havoc_new (Atomic (Acc e_r f Wildcard)) \<omega> RFailure"
-(** others **)
- | InhInhaleExhale: 
-    "\<lbrakk> red_inhale Pr \<Delta> havoc_new A \<omega> res \<rbrakk> \<Longrightarrow> 
-       red_inhale Pr \<Delta> havoc_new (InhaleExhale A B) \<omega> res"
-  | InhPureNormalMagic: 
-    "\<lbrakk> wd_pure_exp_total Pr \<Delta> CInhale e \<omega>;  
-      Pr, \<Delta> \<turnstile> \<langle>e; \<omega>\<rangle> [\<Down>]\<^sub>t Val (VBool b) \<rbrakk> \<Longrightarrow>
-      red_inhale Pr \<Delta> havoc_new (Atomic (Pure e)) \<omega> (if b then RNormal \<omega> else RMagic)"
-  | InhPureFail: 
-    "\<lbrakk> \<not>wd_pure_exp_total Pr \<Delta> CInhale e \<omega> \<rbrakk> \<Longrightarrow>
-      red_inhale Pr \<Delta> havoc_new (Atomic (Pure e)) \<omega> RFailure"
-
+(*
 lemma InhPureNormal:
   assumes "wd_pure_exp_total Pr \<Delta> CInhale e \<omega>" and
           "Pr, \<Delta> \<turnstile> \<langle>e; \<omega>\<rangle> [\<Down>]\<^sub>t Val (VBool True)"
         shows "red_inhale Pr \<Delta> havoc_new (Atomic (Pure e)) \<omega> (RNormal \<omega>)"
   using InhPureNormalMagic[OF assms]
   by simp
+*)
 
-definition get_valid_locs :: "'a full_total_state \<Rightarrow> heap_loc set"
-  where "get_valid_locs \<omega> = {l |l. pgt (get_mask_total_full \<omega> l) pnone}"
+datatype 'a exhale_result = ExhaleNormal "mask \<times> 'a predicate_mask" | ExhaleFailure
 
-datatype exhale_result = ExhaleNormal mask | ExhaleFailure
+fun exh_if_total :: "bool \<Rightarrow> mask \<times> 'a predicate_mask \<Rightarrow> 'a exhale_result"  where
+  "exh_if_total False _ = ExhaleFailure"
+| "exh_if_total True m = ExhaleNormal m"
 
-inductive red_exhale :: "program \<Rightarrow> 'a interp \<Rightarrow> 'a full_total_state \<Rightarrow> assertion \<Rightarrow> mask \<Rightarrow> exhale_result \<Rightarrow> bool"
+
+definition exhale_perm_single :: "mask \<Rightarrow> heap_loc \<Rightarrow> prat option \<Rightarrow> mask set"
+  where "exhale_perm_single m l p_opt =
+      {m'| m' q. 
+               (p_opt = None \<longrightarrow> pgt q pnone) \<and>
+               option_fold ((=) q) (q \<noteq> pnone \<and> pgt (m l) q) p_opt \<and>
+               m' = m(l := psub (m l) q)
+       }"
+
+
+inductive red_exhale :: "program \<Rightarrow> 'a interp \<Rightarrow> 'a full_total_state \<Rightarrow> assertion \<Rightarrow> mask \<times> 'a predicate_mask \<Rightarrow> 'a  exhale_result \<Rightarrow> bool"
   for Pr :: program and \<Delta> :: "'a interp" and \<omega>0 :: "'a full_total_state"
-  where 
+  where
+
+\<comment>\<open>exhale acc(e.f, p)\<close>
+    ExhAcc: 
+    "\<lbrakk> \<omega> = update_mask_total_full \<omega>0 m;
+       Pr, \<Delta>, Some (get_valid_locs \<omega>0) \<turnstile> \<langle>e_r; \<omega>\<rangle> [\<Down>]\<^sub>t Val (VRef r); 
+       Pr, \<Delta>, Some (get_valid_locs \<omega>0) \<turnstile> \<langle>e_p; \<omega>\<rangle> [\<Down>]\<^sub>t Val (VPerm p);
+       a = the_address r \<rbrakk> \<Longrightarrow>
+       red_exhale Pr \<Delta> \<omega>0 (Atomic (Acc e_r f (PureExp e_p))) (m,pm) 
+                           (exh_if_total (p \<ge> 0 \<and> pgte (m(a,f)) (Abs_prat p) \<and> r \<noteq> Null) (m( (a,f) := psub (m (a,f)) (Abs_prat p)),pm)) "
+
+ \<comment>\<open>Exhaling wildcard removes some non-zero permission that this is less than the current permission held\<close>
+  | ExhAccWildcard:
+    "\<lbrakk> \<omega> = update_mask_total_full \<omega>0 m;
+       Pr, \<Delta>, Some (get_valid_locs \<omega>0) \<turnstile> \<langle>e_r; \<omega>\<rangle> [\<Down>]\<^sub>t Val (VRef r);
+       q \<in> {p. p \<noteq> pnone \<and> pgt (m(a,f)) q} \<rbrakk> \<Longrightarrow>
+       red_exhale Pr \<Delta> \<omega>0 (Atomic (Acc e_r f Wildcard)) (m,pm) 
+                           (exh_if_total (m(a,f) \<noteq> pnone \<and> r \<noteq> Null) 
+                                         (m( (a,f) := q),pm))"
+
+\<comment>\<open>exhale acc(P(es), p)\<close>
+  | ExhAccPred:
+     "\<lbrakk> \<omega> = update_mask_total_full \<omega>0 m;
+       red_pure_exps_total Pr \<Delta> (Some (get_valid_locs \<omega>)) e_args \<omega> (map Val v_args);
+       Pr, \<Delta>, Some (get_valid_locs \<omega>0) \<turnstile> \<langle>e_p; \<omega>\<rangle> [\<Down>]\<^sub>t Val (VPerm p) \<rbrakk> \<Longrightarrow>
+      red_exhale Pr \<Delta> \<omega>0 (Atomic (AccPredicate pred_id e_args (PureExp e_p))) (m,pm)
+              (exh_if_total (p \<ge> 0 \<and> pgte (pm(pred_id, v_args)) (Abs_prat p) \<and> r \<noteq> Null) 
+                            (m, pm( (pred_id, v_args) := psub (pm (pred_id, v_args)) (Abs_prat p))))"
+  | ExhAccPredWildcard:
+    "\<lbrakk> \<omega> = update_mask_total_full \<omega>0 m;
+       red_pure_exps_total Pr \<Delta> (Some (get_valid_locs \<omega>)) e_args \<omega> (map Val v_args);
+       q \<in> {p. p \<noteq> pnone \<and> pgt (m(a,f)) q} \<rbrakk> \<Longrightarrow>
+       red_exhale Pr \<Delta> \<omega>0 (Atomic (AccPredicate pred_id e_args Wildcard)) (m,pm) 
+                           (exh_if_total (m(a,f) \<noteq> pnone)
+                                         (m, pm ( (pred_id, v_args) := q )))"
+
+\<comment>\<open>exhale other cases\<close>
+  | ExhPure:
+    "\<lbrakk> \<omega> = update_mask_total_full \<omega>0 m; 
+       Pr, \<Delta>, Some (get_valid_locs \<omega>0) \<turnstile> \<langle>e; \<omega>\<rangle> [\<Down>]\<^sub>t Val (VBool b) \<rbrakk> \<Longrightarrow>
+       red_exhale Pr \<Delta> \<omega>0 (Atomic (Pure e)) (m,pm) (if b then ExhaleNormal (m,pm) else ExhaleFailure)"
+  | SubAtomicFailure: 
+    "\<lbrakk> e \<in> sub_expressions_atomic A ;
+      Pr, \<Delta>, Some (get_valid_locs \<omega>0) \<turnstile> \<langle>e; \<omega>\<rangle> [\<Down>]\<^sub>t VFailure  \<rbrakk> \<Longrightarrow> 
+       red_exhale Pr \<Delta> \<omega>0 (Atomic A) (m,pm) ExhaleFailure"
 
 \<comment>\<open>exhale A && B\<close>
-   ExhSepNormal: 
-   "\<lbrakk> red_exhale Pr \<Delta> \<omega>0 A m (ExhaleNormal m''); 
-      red_exhale Pr \<Delta> \<omega>0 B m'' res\<rbrakk> \<Longrightarrow>
-      red_exhale Pr \<Delta> \<omega>0 (A && B) m res"
+  |  ExhSepNormal: 
+   "\<lbrakk> red_exhale Pr \<Delta> \<omega>0 A m_pm (ExhaleNormal m_pm'); 
+      red_exhale Pr \<Delta> \<omega>0 B m_pm' res\<rbrakk> \<Longrightarrow>
+      red_exhale Pr \<Delta> \<omega>0 (A && B) m_pm res"
  | ExhSepFailureMagic: 
-   "\<lbrakk> red_exhale Pr \<Delta> \<omega>0 A m ExhaleFailure \<rbrakk> \<Longrightarrow>
-      red_exhale Pr \<Delta> \<omega>0 (A && B) m ExhaleFailure"
+   "\<lbrakk> red_exhale Pr \<Delta> \<omega>0 A m_pm ExhaleFailure \<rbrakk> \<Longrightarrow>
+      red_exhale Pr \<Delta> \<omega>0 (A && B) m_pm ExhaleFailure"
 
 \<comment>\<open>exhale A \<longrightarrow> B\<close>
  | ExhImpTrue: 
-   "\<lbrakk> \<omega> = update_mask_total_full \<omega>0 m;
-      wd_pure_exp_total Pr \<Delta> (CExhale (get_valid_locs \<omega>0)) e \<omega>; 
-      Pr, \<Delta> \<turnstile> \<langle>e; \<omega>\<rangle> [\<Down>]\<^sub>t Val (VBool True); 
-      red_exhale Pr \<Delta> \<omega>0 A m res \<rbrakk> \<Longrightarrow>
-      red_exhale Pr \<Delta> \<omega>0 (Imp e A) m res" 
+   "\<lbrakk>  \<omega> = update_mask_and_pmask_total_full \<omega>0 (fst m_pm) (snd m_pm);
+      Pr, \<Delta>, Some (get_valid_locs \<omega>0) \<turnstile> \<langle>e; \<omega>\<rangle> [\<Down>]\<^sub>t Val (VBool True); 
+      red_exhale Pr \<Delta> \<omega>0 A m_pm res \<rbrakk> \<Longrightarrow>
+      red_exhale Pr \<Delta> \<omega>0 (Imp e A) m_pm res" 
  | ExhImpFalse:  
-   "\<lbrakk> \<omega> = update_mask_total_full \<omega>0 m;
-      wd_pure_exp_total Pr \<Delta> (CExhale (get_valid_locs \<omega>0)) e \<omega>; 
-      Pr, \<Delta> \<turnstile> \<langle>e; \<omega>\<rangle> [\<Down>]\<^sub>t Val (VBool False) \<rbrakk> \<Longrightarrow> 
-      red_exhale Pr \<Delta> \<omega>0 (Imp e A) m (ExhaleNormal m)"
+   "\<lbrakk> \<omega> = update_mask_and_pmask_total_full \<omega>0 (fst m_pm) (snd m_pm);
+      Pr, \<Delta>, Some (get_valid_locs \<omega>0) \<turnstile> \<langle>e; \<omega>\<rangle> [\<Down>]\<^sub>t Val (VBool False) \<rbrakk> \<Longrightarrow> 
+      red_exhale Pr \<Delta> \<omega>0 (Imp e A) m_pm (ExhaleNormal m_pm)"
  | ExhImpFailure:
-   "\<lbrakk> \<not> wd_pure_exp_total Pr \<Delta> (CExhale (get_valid_locs \<omega>0)) e (update_mask_total_full \<omega>_orig m) \<rbrakk> \<Longrightarrow> 
-     red_exhale Pr \<Delta> \<omega>0 (Imp e A) m ExhaleFailure"
-
-\<comment>\<open>exhale acc(e.f, p)\<close>
- | ExhAcc: 
-    "\<lbrakk> \<omega> = update_mask_total_full \<omega>0 m;
-       Pr, \<Delta> \<turnstile> \<langle>e_r; \<omega>\<rangle> [\<Down>]\<^sub>t Val (VRef (Address a)); Pr, \<Delta> \<turnstile> \<langle>e_p; \<omega>\<rangle> [\<Down>]\<^sub>t Val (VPerm p); 
-       p \<ge> 0; 
-       pgte (m(a,f)) (Abs_prat p);
-       wd_pure_exp_total Pr \<Delta> (CExhale locs) e_r \<omega>;
-       wd_pure_exp_total Pr \<Delta> (CExhale locs) e_p \<omega>;
-       m' = m( (a,f) := Abs_prat ( (Rep_prat (m((a, f)))) - p) ) \<rbrakk> \<Longrightarrow>
-       red_exhale Pr \<Delta> \<omega>0 (Atomic (Acc e_r f (PureExp e_p))) m (ExhaleNormal m')"
-  | ExhAccFail1: 
-    "\<lbrakk> Pr, \<Delta> \<turnstile> \<langle>e_r; \<omega>\<rangle> [\<Down>]\<^sub>t Val (VRef r); Pr, \<Delta> \<turnstile> \<langle>e_p; \<omega>\<rangle> [\<Down>]\<^sub>t Val (VPerm p); 
-      (r = Null \<or> \<not>wd_pure_exp_total Pr \<Delta> (CExhale locs) e_r \<omega> \<or> \<not>wd_pure_exp_total Pr \<Delta> (CExhale locs) e_p \<omega> \<or> p < 0)\<rbrakk> \<Longrightarrow>
-      red_exhale Pr \<Delta> \<omega>0 (Atomic (Acc e_r f (PureExp e_p))) m ExhaleFailure"
-  | ExhAccFail2:
-    "\<lbrakk> \<omega> = update_mask_total_full \<omega>0 m;
-       Pr, \<Delta> \<turnstile> \<langle>e_r; \<omega>\<rangle> [\<Down>]\<^sub>t Val (VRef (Address a));
-       Pr, \<Delta> \<turnstile> \<langle>e_p; \<omega>\<rangle> [\<Down>]\<^sub>t Val (VPerm p);
-       wd_pure_exp_total Pr \<Delta> (CExhale locs) e_r \<omega>;
-       wd_pure_exp_total Pr \<Delta> (CExhale locs) e_p \<omega>;
-       p \<ge> 0; 
-       \<not> (pgte (m(a,f)) (Abs_prat p)) \<rbrakk> \<Longrightarrow>
-       red_exhale Pr \<Delta> \<omega>0 (Atomic (Acc e_r f (PureExp e_p))) m ExhaleFailure"
-
-\<comment>\<open>exhale acc(e.f, wildcard)\<close>
- \<comment>\<open>Exhaling wildcard removes some non-zero permission this is less than the current permission held\<close>
-  | ExhAccWildcard:
-    "\<lbrakk> \<omega> = update_mask_total_full \<omega>0 m;
-       Pr, \<Delta> \<turnstile> \<langle>e_r; \<omega>\<rangle> [\<Down>]\<^sub>t Val (VRef (Address a));
-       p > 0; 
-       pgt (m(a,f)) (Abs_prat p);
-       wd_pure_exp_total Pr \<Delta> (CExhale locs) e_r \<omega>;
-       m' = m( (a,f) := Abs_prat ( (Rep_prat (m((a, f)))) - p) ) \<rbrakk> \<Longrightarrow>
-       red_exhale Pr \<Delta> \<omega>0 (Atomic (Acc e_r f Wildcard)) m (ExhaleNormal m')"
-  | ExhAccWildcardFail1:
-    "\<lbrakk> Pr, \<Delta> \<turnstile> \<langle>e_r; \<omega>\<rangle> [\<Down>]\<^sub>t Val (VRef r); 
-      (r = Null \<or> \<not>wd_pure_exp_total Pr \<Delta> (CExhale locs) e_r \<omega>)\<rbrakk> \<Longrightarrow>
-      red_exhale Pr \<Delta> \<omega>0 (Atomic (Acc e_r f Wildcard)) m ExhaleFailure"
-  | ExhAccWildcardFail2:
-    "\<lbrakk> \<omega> = update_mask_total_full \<omega>0 m;
-       Pr, \<Delta> \<turnstile> \<langle>e_r; \<omega>\<rangle> [\<Down>]\<^sub>t Val (VRef (Address a));
-       wd_pure_exp_total Pr \<Delta> (CExhale locs) e_r \<omega>;
-       (m(a,f)) = pnone \<rbrakk> \<Longrightarrow>
-      red_exhale Pr \<Delta> \<omega>0 (Atomic (Acc e_r f Wildcard)) m ExhaleFailure"
- 
-\<comment>\<open>exhale other cases\<close>
-  | ExhInhaleExhale: 
-    "\<lbrakk> red_exhale Pr \<Delta> \<omega>0 B m res \<rbrakk> \<Longrightarrow> 
-       red_exhale Pr \<Delta> \<omega>0 (InhaleExhale A B) m res"  
-  | ExhPure:
-    "\<lbrakk> \<omega> = update_mask_total_full \<omega>0 m; 
-       wd_pure_exp_total Pr \<Delta> (CExhale locs) e \<omega>;  
-       Pr, \<Delta> \<turnstile> \<langle>e; \<omega>\<rangle> [\<Down>]\<^sub>t Val (VBool b) \<rbrakk> \<Longrightarrow>
-       red_exhale Pr \<Delta> \<omega>0 (Atomic (Pure e)) m (if b then ExhaleNormal m else ExhaleFailure)"
-  | ExhPureFail:
-    "\<lbrakk> \<omega> = update_mask_total_full \<omega>0 m; 
-       \<not> (wd_pure_exp_total Pr \<Delta> (CExhale locs) e \<omega>) \<rbrakk> \<Longrightarrow>
-       red_exhale Pr \<Delta> \<omega>0 (Atomic (Pure e)) m ExhaleFailure"
+   "\<lbrakk> \<omega> = update_mask_and_pmask_total_full \<omega>0 (fst m_pm) (snd m_pm); 
+      Pr, \<Delta>, Some (get_valid_locs \<omega>0) \<turnstile> \<langle>e; \<omega>\<rangle> [\<Down>]\<^sub>t VFailure \<rbrakk> \<Longrightarrow> 
+     red_exhale Pr \<Delta> \<omega>0 (Imp e A) m_pm ExhaleFailure"
 
 record conf =
   havoc_inhale :: bool
@@ -198,8 +110,8 @@ record conf =
 definition havoc_undef_locs :: "'a full_total_state \<Rightarrow> mask \<Rightarrow> 'a full_total_state set"
   where "havoc_undef_locs \<omega> m = {\<omega>'| \<omega>'. \<forall>l. pgt (m l) pnone \<longrightarrow> get_heap_total_full \<omega> l = get_heap_total_full \<omega>' l}"
 *)
-definition havoc_undef_locs :: "'a total_heap \<Rightarrow> mask \<Rightarrow> 'a total_heap set"
-  where "havoc_undef_locs h m = {h' | h'. \<forall>l. pgt (m l) pnone \<longrightarrow> h' l = h l}"
+definition havoc_undef_locs :: "'a total_heap \<Rightarrow> 'a predicate_heap \<Rightarrow> mask \<Rightarrow> 'a predicate_mask \<Rightarrow> 'a total_heap set"
+  where "havoc_undef_locs h m pm = {h' | h'. \<forall>l. pgt (m l) pnone \<longrightarrow> h' l = h l}"
 
 definition exhale_state :: "'a full_total_state \<Rightarrow> mask \<Rightarrow> 'a full_total_state set"
   where "exhale_state \<omega> m = {\<omega>' | \<omega>'. get_store_total \<omega>' = get_store_total \<omega> \<and>
